theories/Lang/Vec.v
@@ -1,0 +1,999 @@
+From Coq Require Import
+     Program
+     List
+     Classes.Morphisms
+     Logic.FinFun
+     Logic.FunctionalExtensionality
+     Logic.IndefiniteDescription
+     micromega.Lia
+     Init.Specif
+     Fin.
+
+From Equations Require Import Equations.
+
+From CTree Require Import
+  CTree.Core
+  Equ
+  SBisim
+  CTree.Interp.State.
+
+Import ListNotations.
+Import CTreeNotations.
+
+Local Open Scope ctree_scope.
+
+Generalizable All Variables.
+
+Notation pwr := (pointwise_relation _).
+Notation vec n T := (fin n -> T).
+Notation vec' n T := (vec (S n) T).
+
+Section Vectors.
+  Context {thread : Type}.
+  Notation vec n := (vec n thread).
+  Notation vec' n := (vec' n thread).
+
+  (** Removing an element from a [vec] *)
+  Definition remove_front_vec {n : nat} (v : vec' n) : vec n :=
+    fun i => v (FS i).
+
+  #[global] Instance remove_front_vec_relation n P :
+    Proper (pwr P ==> pwr P) (@remove_front_vec n).
+  Proof.
+    repeat intro. apply H.
+  Qed.
+
+  Equations remove_vec {n : nat} (v : vec' n) (i : fin (S n)) : vec n :=
+    remove_vec v F1     i'      := remove_front_vec v i';
+    remove_vec v (FS i) F1      := v F1;
+    remove_vec v (FS i) (FS i') := remove_vec (remove_front_vec v) i i'.
+  Transparent remove_vec.
+
+  #[global] Instance remove_vec_relation n P :
+    Proper (pwr P ==> eq ==> pwr P) (@remove_vec n).
+  Proof.
+    intros v1 v2 Pv ? i ?. subst.
+    depind i; [apply remove_front_vec_relation; auto |].
+    intro i'. destruct i'; cbn; auto.
+    apply IHi; auto.
+    repeat intro. apply remove_front_vec_relation; auto.
+  Qed.
+
+  Lemma remove_vec_remove_vec_front n (v : vec (S (S n))) i i' :
+    remove_vec (remove_front_vec v) i i' = remove_front_vec (remove_vec v (FS i)) i'.
+  Proof.
+    depind i; cbn; auto.
+  Qed.
+
+  (* before the element removed, the same index works *)
+  Lemma remove_vec_index_before {n} (v : vec' n) i j
+        (Hi : i < S n) (Hji : j < i) (Hj : j < S n) (Hj' : j < n) :
+    v (of_nat_lt Hj) = (remove_vec v (of_nat_lt Hi)) (of_nat_lt Hj').
+  Proof.
+    revert n v j Hi Hj Hj' Hji. induction i; intros; auto. inv Hji.
+    destruct n. inv Hj'. destruct j; auto. cbn.
+    erewrite <- IHi; auto. lia.
+  Qed.
+
+  (* after the element removed, we need to subtract one from the index *)
+  Lemma remove_vec_index_after {n} (v : vec' n) i j
+        (Hi : i < S n) (Hji : j > i) (Hj : S j < S n) (Hj' : j < n) (* S j to j *) :
+    v (of_nat_lt Hj) = (remove_vec v (of_nat_lt Hi)) (of_nat_lt Hj').
+  Proof.
+    revert n v i Hi Hji Hj Hj'. induction j; intros. inv Hji.
+    destruct i.
+    - destruct n. inv Hj'. cbn. unfold remove_front_vec. erewrite of_nat_ext. reflexivity.
+    - destruct n. inv Hj'. cbn. erewrite <- IHj; eauto. lia.
+  Qed.
+
+  (* at the element removed, we also subtract one. TODO: can we unify this with prev lemma? *)
+  Lemma remove_vec_index_eq {n} (v : vec' n) i j
+        (Hi : i < S n) (Hji : j = i) (Hj : S j < S n) (Hj' : j < n) :
+    v (of_nat_lt Hj) = (remove_vec v (of_nat_lt Hi)) (of_nat_lt Hj').
+  Proof.
+    revert n v j Hi Hj Hj' Hji. induction i; intros; auto.
+    - destruct n. inv Hj'. subst. reflexivity.
+    - destruct n. inv Hj'. subst. cbn.
+      erewrite <- IHi; auto.
+  Qed.
+
+  Definition remove_vec_helper n n' (v : vec n) (i : fin n) (H : n = S n')
+    : vec n'.
+    subst. apply remove_vec; eauto.
+  Defined.
+
+
+  (** Replacing an element in a [vec] *)
+  Definition replace_vec {n : nat} (v : vec n) (i : fin n) (t : thread) : vec n :=
+    fun i' => if Fin.eqb i i' then t else v i'.
+
+  Lemma replace_vec_unary t1 t2 :
+    replace_vec (fun _: fin 1 => t1) F1 t2 = (fun _ => t2).
+  Proof.
+    apply functional_extensionality. intros. dependent destruction x; auto. inv x.
+  Qed.
+
+  Lemma remove_front_vec_replace_vec n (v : vec' n) i t :
+    remove_front_vec (replace_vec v (FS i) t) =
+      replace_vec (remove_front_vec v) i t.
+  Proof. reflexivity. Qed.
+
+  Lemma remove_vec_replace_vec_eq {n} (v : vec' n) i t :
+    remove_vec v i = remove_vec (replace_vec v i t) i.
+  Proof.
+    dependent induction i.
+    - unfold remove_vec. unfold remove_front_vec. cbn. reflexivity.
+    - unfold remove_vec. cbn. apply functional_extensionality. intros.
+      dependent destruction x; auto.
+      erewrite IHi; eauto.
+  Qed.
+
+  Lemma remove_vec_helper_replace_vec_eq {n n'} (v : vec n) i t H :
+    remove_vec_helper n n' v i H = remove_vec_helper n n' (replace_vec v i t) i H.
+  Proof.
+    subst. cbn. eapply remove_vec_replace_vec_eq.
+  Qed.
+
+  #[global] Instance replace_vec_relation n P :
+    Proper (pwr P ==> eq ==> P ==> pwr P) (@replace_vec n).
+  Proof.
+    unfold replace_vec. repeat intro. subst. destruct (Fin.eqb y0 a); auto.
+  Qed.
+
+  Lemma replace_vec_twice n (v : vec n) i t1 t2 :
+    replace_vec (replace_vec v i t1) i t2 = replace_vec v i t2.
+  Proof.
+    unfold replace_vec. apply functional_extensionality. intro.
+    destruct (Fin.eqb i x) eqn:?; auto.
+  Qed.
+
+  Lemma replace_vec_eq n (v : vec n) i t :
+    (replace_vec v i t) i = t.
+  Proof.
+    unfold replace_vec.
+    assert (i = i) by reflexivity. apply Fin.eqb_eq in H. rewrite H.
+    reflexivity.
+  Qed.
+
+  Lemma replace_vec_neq n (v : vec n) i1 i2 t :
+    i1 <> i2 ->
+    (replace_vec v i1 t) i2 = v i2.
+  Proof.
+    intros.
+    unfold replace_vec.
+    destruct (Fin.eqb i1 i2) eqn:?.
+    - apply Fin.eqb_eq in Heqb. contradiction.
+    - reflexivity.
+  Qed.
+
+  (** Adding an element to the front of a [vec] *)
+  Equations cons_vec {n : nat} (t : thread) (v : vec n) : vec' n :=
+    cons_vec t v F1      := t;
+    cons_vec t v (FS i)  := v i.
+  Transparent cons_vec.
+
+  #[global] Instance cons_vec_relation n P :
+    Proper (P ==> pwr P ==> pwr P) (@cons_vec n).
+  Proof.
+    unfold cons_vec. repeat intro. depind a; cbn; auto.
+  Qed.
+
+  Lemma remove_vec_cons_1 t1 t2 :
+    (remove_vec (cons_vec t1 (fun _ : fin 1 => t2)) F1) = (fun _ => t2).
+  Proof.
+    apply functional_extensionality. intros i. dependent destruction i; [| inv i].
+    simp remove_vec. unfold remove_front_vec. simp cons_vec. reflexivity.
+  Qed.
+
+  Lemma remove_vec_cons_2 t1 t2 :
+    (remove_vec (cons_vec t1 (fun _ : fin 1 => t2)) (FS F1)) = (fun _ => t1).
+  Proof.
+    apply functional_extensionality. intros i. dependent destruction i; [| inv i].
+    simp remove_vec. simp cons_vec. reflexivity.
+  Qed.
+
+  Lemma replace_vec_cons_1 t1 t2 t :
+    (replace_vec (cons_vec t1 (fun _ : fin 1 => t2)) F1 t) =
+      (cons_vec t (fun _ : fin 1 => t2)).
+  Proof.
+    apply functional_extensionality. intros i. dependent destruction i; reflexivity.
+  Qed.
+
+  Lemma replace_vec_cons_2 t1 t2 t :
+    (replace_vec (cons_vec t1 (fun _ : fin 1 => t2)) (FS F1) t) =
+      (cons_vec t1 (fun _ : fin 1 => t)).
+  Proof.
+    apply functional_extensionality. intros i. dependent destruction i; cbn.
+    - reflexivity.
+    - dependent destruction i; [| inv i]. cbn. simp cons_vec. reflexivity.
+  Qed.
+
+  Lemma of_nat_lt_sig1_neq_1 n1 n2 n (H1 : n1 < n) (H2 : n2 < n) :
+    of_nat_lt H1 <> of_nat_lt H2 ->
+    n1 <> n2.
+  Proof.
+    repeat intro. subst. apply H. apply of_nat_ext.
+  Qed.
+
+  Lemma of_nat_lt_sig1_neq_2 n1 n2 n (H1 : n1 < n) (H2 : n2 < n) :
+    n1 <> n2 ->
+    of_nat_lt H1 <> of_nat_lt H2.
+  Proof.
+    revert n2 n H1 H2. induction n1; intros; auto.
+    - destruct n2; auto. destruct n; [inv H2 |]. intro. inv H0.
+    - destruct n; [inv H2 |]. destruct n2.
+      + intro. inv H0.
+      + cbn. intro. inv H0. invert. eapply (IHn1 n2).
+        * intro. subst. contradiction.
+        * apply x.
+  Qed.
+
+  Lemma of_nat_lt_sig1_neq n1 n2 n (H1 : n1 < n) (H2 : n2 < n) :
+    n1 <> n2 <->
+      of_nat_lt H1 <> of_nat_lt H2.
+  Proof.
+    split. apply of_nat_lt_sig1_neq_2. apply of_nat_lt_sig1_neq_1.
+  Qed.
+
+  Definition cons_permutation {n} (p : fin n -> fin n) :
+    {
+      p' : (fin (S n) -> fin (S n)) &
+             p' F1 = F1 /\ forall i, p' (FS i) = FS (p i)
+    }.
+    eexists. Unshelve.
+    2: {
+      intro i.
+      dependent destruction i.
+      - apply F1.
+      - apply (FS (p i)).
+    }
+    split; auto.
+  Defined.
+
+  Lemma cons_permutation_correct {n} (p q : fin n -> fin n)
+        (Hpq : forall i, p (q i) = i)
+        (Hqp : forall i, q (p i) = i) :
+    let p' := projT1 (cons_permutation p) in
+    let q' := projT1 (cons_permutation q) in
+    (forall i, p' (q' i) = i) /\ (forall i, q' (p' i) = i).
+  Proof.
+    destruct (cons_permutation p) as (p' & Hp1 & Hp2).
+    destruct (cons_permutation q) as (q' & Hq1 & Hq2).
+    cbn in *. split.
+    - intro i. dependent destruction i.
+      + rewrite Hq1, Hp1. auto.
+      + rewrite Hq2, Hp2, Hpq. auto.
+    - intro i. dependent destruction i.
+      + rewrite Hp1, Hq1. auto.
+      + rewrite Hp2, Hq2, Hqp. auto.
+  Qed.
+
+End Vectors.
+
+Section Ordering.
+  Variant ordering := LT | EQ | GT.
+
+  Fixpoint order {m n} (p : fin m) (q : fin n) : ordering :=
+    match p, q with
+    | F1, F1 => EQ
+    | F1, _ => LT
+    | _, F1 => GT
+    | FS p', FS q' => order p' q'
+    end.
+
+  (** General [order] lemmas *)
+
+  Lemma order_reflexive {n} (p : fin n) :
+    order p p = EQ.
+  Proof.
+    depind p; auto.
+  Qed.
+
+  Lemma order_transitive {m n o} (p : fin m) (q : fin n) (r : fin o) l :
+    order p q = l ->
+    order q r = l ->
+    order p r = l.
+  Proof.
+    destruct l.
+    {
+      revert n o q r.
+      depind p; intros; auto.
+      - dependent destruction q; auto. dependent destruction r; auto. inv H0.
+      - dependent destruction q; auto; [inv H |].
+        dependent destruction r; auto. cbn in *. eapply IHp; eauto.
+    }
+    {
+      revert n o q r.
+      depind p; intros; auto.
+      - dependent destruction q; auto. dependent destruction r; auto.
+      - dependent destruction q; auto; [inv H |].
+        dependent destruction r; auto. cbn in *. eapply IHp; eauto.
+    }
+    {
+      revert n o q r.
+      depind p; intros; auto.
+      - dependent destruction q; auto. dependent destruction r; auto. inv H.
+      - dependent destruction q.
+        + dependent destruction r; auto; inv H0.
+        + dependent destruction r; auto. cbn in *. eapply IHp; eauto.
+    }
+  Qed.
+
+  Lemma order_flip {m n} (p : fin m) (q : fin n) :
+    order p q = LT <-> order q p = GT.
+  Proof.
+    split.
+    {
+      revert n q.
+      depind p; dependent destruction q; auto.
+      - intros. inv H.
+      - cbn. eapply IHp.
+    }
+    {
+      revert n q.
+      depind p; dependent destruction q; auto.
+      - intros. inv H.
+      - cbn. eapply IHp.
+    }
+  Qed.
+
+  Lemma order_eq {n} (p q : fin n) :
+    order p q = EQ -> p = q.
+  Proof.
+    depind p; intros; dependent destruction q; inv H; auto.
+    f_equal. auto.
+  Qed.
+
+
+  Lemma order_EQ_FS {m n} (p : fin m) (q : fin n) :
+    order p q = EQ -> order (FS p) q = GT.
+  Proof.
+    revert n q.
+    depind p.
+    - intros. dependent destruction q; inv H; auto.
+    - intros. dependent destruction q. inv H. cbn in H. apply IHp; auto.
+  Qed.
+
+  Lemma order_GT_FS {m n} (p : fin m) (q : fin n) :
+    order p q = GT -> order (FS p) q = GT.
+  Proof.
+    revert n q.
+    depind p.
+    - intros. dependent destruction q; inv H; auto.
+    - intros. dependent destruction q; auto. cbn in H. apply IHp; auto.
+  Qed.
+
+  Lemma order_FS_LT {n} (i : fin n) :
+    order i (FS i) = LT.
+  Proof.
+    induction i; auto.
+  Qed.
+
+  Lemma order_FS_GT_inv {m n} (p : fin m) (q : fin n) :
+    order (FS p) q = GT ->
+    order p q = EQ \/ order p q = GT.
+  Proof.
+    intros. generalize dependent n. depind p; intros.
+    - dependent destruction q.
+      + left; auto.
+      + dependent destruction q; inv H.
+    - dependent destruction q.
+      + right; auto.
+      + cbn in H. destruct (IHp _ q H); auto.
+  Qed.
+
+  Lemma order_cases {m n} (p : fin m) (q : fin n) :
+    {order p q = LT} + {order p q = EQ} + {order p q = GT}.
+  Proof.
+    destruct (order p q); intuition.
+  Qed.
+
+  (** For converting a value of type [fin (S (S n))] into one of type [fin (S n)] *)
+  Equations not_highest {n} (p q : fin (S (S n))) (H: order p q = LT) : fin (S n) :=
+    not_highest F1 q H := F1 ;
+    not_highest (FS p') F1 H := _;
+    @not_highest 0 (FS p') (FS q') H := _;
+    @not_highest (S n) (FS p') (FS q') H := FS (not_highest p' q' _).
+  
+  Lemma not_highest_FS {n} (p q : fin (S (S n))) H H' :
+    (not_highest (FS p) (FS q) H) = FS (not_highest p q H').
+  Proof.
+    simp not_highest. f_equal. f_equal. apply proof_irrelevance.
+  Qed.
+
+  Lemma order_not_highest {n} (p q r : fin (S (S n))) H :
+    order p r = order (not_highest p q H) r.
+  Proof.
+    depind p.
+    - simp not_highest. reflexivity.
+    - dependent destruction q. inv H.
+      destruct n.
+      + cbn in *. depind p. depind q. inv H. inv q. inv p.
+      + cbn in H. rewrite not_highest_FS with (H':=H).
+        cbn in *. dependent destruction r; auto.
+  Qed.
+
+  Lemma order_not_highest_EQ {n} (p q : fin (S (S n))) H :
+    order (not_highest p q H) p = EQ.
+  Proof.
+    depind p; auto.
+    - simp not_highest. auto.
+    - dependent destruction q. inv H.
+      destruct n.
+      + cbn in H.
+        dependent destruction p. 2: inv p.
+        dependent destruction q. inv H. inv q.
+      + simp not_highest. cbn. apply IHp; auto.
+  Qed.
+
+  (** view a [fin n] as a [fin (S n)] *)
+  Equations fin_S {n} (i : fin n) : fin (S n) :=
+    fin_S F1 := F1;
+    fin_S (FS i') := FS (fin_S i').
+
+  Lemma order_fin_S_EQ {n} (i : fin n) : order i (fin_S i) = EQ.
+  Proof.
+    depind i; auto.
+  Qed.
+
+  Lemma order_fin_S m n (p : fin m) (q : fin n) : order p q = order (fin_S p) q.
+  Proof.
+    intros. revert n q. depind p.
+    - reflexivity.
+    - dependent destruction q.
+      + reflexivity.
+      + cbn. rewrite IHp. reflexivity.
+  Qed.
+
+  Lemma fin_S_not_highest {n} (p q : fin (S (S n))) H : fin_S (not_highest p q H) = p.
+  Proof.
+    depind p; cbn; auto.
+    - simp not_highest. simp fin_S. reflexivity.
+    - dependent destruction q. inv H.
+      destruct n. cbn in H.
+      dependent destruction p. dependent destruction q. inv H. inv q. inv p.
+      simp not_highest. simp fin_S. f_equal. apply IHp; auto.
+  Qed.
+
+  Lemma not_highest_fin_S {n} (p : fin (S n)) q H : (not_highest (fin_S p) q H) = p.
+  Proof.
+    destruct n.
+    { dependent destruction p. auto. inv p. }
+    depind p; auto.
+    dependent destruction q. inv H.
+    revert H. simp fin_S. intro.
+    destruct n; auto.
+    - cbn in *. dependent destruction p. 2: inv p. auto.
+    - simp not_highest. f_equal. auto.
+  Qed.
+
+  (** p is greater than another value, so we can subtract one *)
+  Equations subtract_one {n} (p q : fin (S n)) (H: order p q = GT) : fin n :=
+  subtract_one F1 q H := _;
+  subtract_one (FS p') q H := p'.
+  Next Obligation.
+    intros. dependent destruction q; inv H.
+  Defined.
+
+  Lemma subtract_one_FS {n} p (q : fin (S n)) H :
+    subtract_one (FS p) q H = p.
+  Proof.
+    reflexivity.
+  Qed.
+
+  Lemma FS_subtract_one {n} (p q : fin (S n)) H :
+    FS (subtract_one p q H) = p.
+  Proof.
+    dependent destruction p.
+    - dependent destruction q; inv H.
+    - reflexivity.
+  Qed.
+
+  Lemma order_subtract_one_GT {n} (p q : fin (S n)) (H : order p q = GT) :
+    order p (subtract_one p q H) = GT.
+  Proof.
+    dependent destruction p.
+    - dependent destruction q; inv H.
+    - destruct n. inv p. rewrite subtract_one_FS. apply order_flip. apply order_FS_LT.
+  Qed.
+
+  Lemma order_subtract_one_GT_inv {n} (p q r : fin (S n)) H :
+    order p q = GT ->
+    order (subtract_one p r H) q = EQ \/ order (subtract_one p r H) q = GT.
+  Proof.
+    intros.
+    dependent destruction p.
+    - dependent destruction q; inv H0.
+    - destruct n. inv p.
+      rewrite subtract_one_FS. apply order_FS_GT_inv; auto.
+  Qed.
+
+  Lemma order_subtract_one_LT_inv {n} (p q r : fin (S n)) H :
+     order (subtract_one p r H) q = LT ->
+     order p q = EQ \/ order p q = LT.
+  Proof.
+    intros.
+    depind p. dependent destruction r; inv H.
+    destruct n. inv p. specialize (IHp n p eq_refl JMeq_refl).
+    rewrite subtract_one_FS in H0.
+    dependent destruction q. dependent destruction p; inv H0. cbn.
+    dependent destruction p. dependent destruction q; auto.
+    cbn in H0.
+    eapply (IHp q (fin_S p) _ _). Unshelve.
+    - rewrite <- order_flip. rewrite <- order_fin_S. apply order_FS_LT.
+    - rewrite subtract_one_FS. auto.
+  Qed.
+
+  (** lemmas about remove_vec and order *)
+  Lemma remove_vec_index_before' {T n} (v : vec' n T) i j
+    (Hj : order j i = LT) :
+    v (fin_S j) = remove_vec v i j.
+  Proof.
+    revert v j Hj. depind i; intros; auto.
+    - dependent destruction j; inv Hj.
+    - destruct n; [inv j |]. dependent destruction j; auto. cbn. simp fin_S.
+      simp remove_vec. erewrite <- IHi; auto.
+  Qed.
+
+  (* after the element removed, we need to subtract one from the index *)
+  Lemma remove_vec_index_after' {n T} (v : vec' n T) i j
+        (Hj : order j i = GT) :
+    v (FS j) = remove_vec v i j.
+  Proof.
+    revert v i Hj. depind j; intros. dependent destruction i; auto; inv Hj.
+    dependent destruction i.
+    - destruct n. inv j. reflexivity.
+    - destruct n. inv j. simp remove_vec. rewrite <- IHj; auto.
+  Qed.
+
+  (* at the element removed, we also subtract one. TODO: can we unify this with prev lemma? *)
+  Lemma remove_vec_index_eq' {n T} (v : vec' n T) i j
+        (Hj : order j i = EQ) :
+    v (FS j) = remove_vec v i j.
+  Proof.
+    revert v i Hj. depind j; intros. dependent destruction i; auto; inv Hj.
+    dependent destruction i. inv Hj.
+    destruct n. inv j. simp remove_vec. rewrite <- IHj; auto.
+  Qed.
+
+  Ltac cases a b name := destruct (order_cases a b) as [[name | name] | name].
+
+  Definition remove_at_permutation {n} (p : fin' (S n) -> fin' (S n))
+             (r : fin (S (S n)))
+             (Hp : Injective p)
+    :
+    { p' : (fin (S n) -> fin (S n)) &
+             (forall i, match (order_cases i r) with
+                   | inleft (left Hi) =>
+                       (* i < r *)
+                       let pi := p (fin_S i) in
+                       match (order_cases pi (p r)) with
+                       | inleft (left Hpi) => (* p i < p r *)
+                           p' i = not_highest _ _ Hpi
+                       | inleft (right Hpi) => (* p i = p r *)
+                           False
+                       | inright Hpi => (* p i > p r *)
+                           p' i = subtract_one _ _ Hpi
+                       end
+                   | _ =>
+                       (* i >= r *)
+                       let pi := p (FS i) in
+                       match (order_cases pi (p r)) with
+                       | inleft (left Hpi) => (* p (i + 1) < p r *)
+                           p' i = not_highest _ _ Hpi
+                       | inleft (right Hpi) => (* p (i + 1) = p r *)
+                           False
+                       | inright Hpi => (* p (i + 1) > p r *)
+                           p' i = subtract_one _ _ Hpi
+                       end
+                   end)
+    }.
+  Proof.
+    eexists. Unshelve.
+    2: {
+      intro i.
+      cases i r Hi.
+      - (* i < r *)
+        remember (p (fin_S i)) as pi.
+        cases pi (p r) Hpi.
+        + (* p i < p r *)
+          apply (not_highest _ _ Hpi).
+        + (* p i = p r, contradiction *)
+          apply order_eq in Hpi. subst. apply Hp in Hpi. rewrite <- Hpi in Hi.
+          rewrite order_fin_S_EQ in Hi. inv Hi.
+        + (* p i > p r *)
+          apply (subtract_one _ _ Hpi).
+      - (* i = r *)
+        remember (p (FS i)) as pi.
+        cases pi (p r) Hpi.
+        + (* p (i + 1) < p r *)
+          apply (not_highest _ _ Hpi).
+        + (* p (i + 1) = p r, contradiction *)
+          apply order_eq in Hpi. subst. apply Hp in Hpi. rewrite <- Hpi in Hi.
+          rewrite order_FS_LT in Hi. inv Hi.
+        + (* p i > p r *)
+          apply (subtract_one _ _ Hpi).
+      - (* i > r *)
+        remember (p (FS i)) as pi.
+        cases pi (p r) Hpi.
+        + (* p (i + 1) < p r *)
+          apply (not_highest _ _ Hpi).
+        + (* p (i + 1) = p r, contradiction *)
+          apply order_eq in Hpi. subst. apply Hp in Hpi. rewrite <- Hpi in Hi.
+          rewrite order_FS_LT in Hi. inv Hi.
+        + (* p i > p r *)
+          apply (subtract_one _ _ Hpi).
+    }
+    intro i. cbn.
+    cases i r Hi.
+    - (* i < r *)
+      set (pi := p (fin_S i)).
+      cases pi (p r) Hpi; auto.
+      (* equals case is a contradiction *)
+      apply order_eq in Hpi. subst. apply Hp in Hpi. rewrite <- Hpi in Hi.
+      rewrite order_fin_S_EQ in Hi. inv Hi.
+    - (* i = r *)
+      set (pi := p (FS i)).
+      cases pi (p r) Hpi; auto.
+      (* equals case is a contradiction *)
+      apply order_eq in Hpi. subst pi. apply Hp in Hpi. rewrite <- Hpi in Hi.
+      rewrite order_FS_LT in Hi. inv Hi.
+    - (* i > r *)
+      set (pi := p (FS i)).
+      cases pi (p r) Hpi; auto.
+      (* equals case is a contradiction *)
+      apply order_eq in Hpi. subst pi. apply Hp in Hpi. rewrite <- Hpi in Hi.
+      rewrite order_FS_LT in Hi. inv Hi.
+  Qed.
+
+  Lemma bijective_injective {n} (p q : fin n -> fin n)
+        (Hqp: forall i, q (p i) = i) :
+    Injective p.
+  Proof.
+    intros i1 i2 ?. apply (f_equal q) in H. do 2 rewrite Hqp in H. auto.
+  Qed.
+
+  Lemma remove_at_permutation_correct {n} (p q : fin (S (S n)) -> fin (S (S n))) r
+        (Hpq : forall i, p (q i) = i)
+        (Hqp : forall i, q (p i) = i)
+        Hinjp Hinjq :
+    let p' := projT1 (remove_at_permutation p r Hinjp) in
+    let q' := projT1 (remove_at_permutation q (p r) Hinjq) in
+    (forall i, p' (q' i) = i) /\ (forall i, q' (p' i) = i).
+  Proof.
+    destruct (remove_at_permutation p r _) as (p' & Hp).
+    destruct (remove_at_permutation q (p r) _) as (q' & Hq).
+    cbn in *. split.
+    {
+      intro i.
+      specialize (Hq i). rewrite Hqp in Hq.
+      cases i (p r) Hi.
+      - (* i < p r *)
+        cases (q (fin_S i)) r Hqi; try contradiction.
+        + (* q i < r *)
+          specialize (Hp (q' i)). rewrite Hq in *.
+          rewrite fin_S_not_highest, Hpq in Hp.
+          cases (not_highest (q (fin_S i)) r Hqi) r Hqi'.
+          2, 3: rewrite <- order_not_highest in Hqi'; rewrite Hqi in Hqi'; inv Hqi'.
+          cases (fin_S i) (p r) Hi'.
+          2, 3: rewrite order_fin_S in Hi; rewrite Hi' in Hi; inv Hi.
+          rewrite Hp. rewrite not_highest_fin_S. reflexivity.
+        + (* q i > r *)
+          specialize (Hp (q' i)). rewrite Hq in *.
+          rewrite FS_subtract_one in Hp. rewrite Hpq in Hp.
+          cases (subtract_one (q (fin_S i)) r Hqi) r Hqi'.
+          1: { (* q i - 1 < r not possible *)
+            pose proof Hqi as Hqi''. eapply order_subtract_one_GT_inv in Hqi''.
+            destruct Hqi'' as [Hqi'' | Hqi'']; rewrite Hqi' in Hqi''; inv Hqi''.
+          }
+          * (* q i - 1 = r *)
+            cases (fin_S i) (p r) Hi'.
+            2, 3: rewrite order_fin_S in Hi; rewrite Hi' in Hi; inv Hi.
+            rewrite Hp. rewrite not_highest_fin_S. reflexivity.
+          * (* q i - 1 > r *)
+            cases (fin_S i) (p r) Hi'.
+            2, 3: rewrite order_fin_S in Hi; rewrite Hi' in Hi; inv Hi.
+            rewrite Hp. rewrite not_highest_fin_S. reflexivity.
+      - (* i = p r *)
+        cases (q (FS i)) r Hqi; try contradiction.
+        + (* q (i + 1) < r *)
+          specialize (Hp (q' i)). rewrite Hq in *.
+          rewrite fin_S_not_highest, Hpq in Hp.
+          cases (not_highest (q (FS i)) r Hqi) r Hqi'.
+          2, 3: rewrite <- order_not_highest in Hqi'; rewrite Hqi in Hqi'; inv Hqi'.
+          cases (FS i) (p r) Hi'; try contradiction.
+          1: { (* i + 1 < p r is not possible *)
+            rewrite order_fin_S in Hi. apply order_eq in Hi. pose proof Hi' as Hi''.
+            rewrite <- Hi in Hi''. rewrite order_flip in Hi''. rewrite <- order_fin_S in Hi''.
+            rewrite order_FS_LT in Hi''. inv Hi''.
+          }
+          (* i + 1 > p r *)
+          rewrite Hp. rewrite subtract_one_FS. reflexivity.
+        + (* q (i + 1) > r *)
+          specialize (Hp (q' i)). rewrite Hq in *.
+          rewrite FS_subtract_one, Hpq in Hp.
+          cases (subtract_one (q (FS i)) r Hqi) r Hqi'.
+          1: { (* q (i + 1) - 1 < r not possible *)
+            apply order_subtract_one_LT_inv in Hqi'.
+            destruct Hqi' as [Hqi' | Hqi']; rewrite Hqi in Hqi'; inv Hqi'.
+          }
+          * (* q (i + 1) - 1 = r *)
+            cases (FS i) (p r) Hi'; try contradiction.
+            1: { (* i + 1 < p r not possible *)
+              rewrite order_fin_S in Hi. apply order_eq in Hi. pose proof Hi' as Hi''.
+              rewrite <- Hi in Hi''. rewrite order_flip in Hi''.
+              rewrite <- order_fin_S in Hi''. rewrite order_FS_LT in Hi''. inv Hi''.
+            }
+            (* i + 1 > p r *)
+            rewrite Hp. rewrite subtract_one_FS. reflexivity.
+          * (* q (i + 1) - 1 > r *)
+            cases (FS i) (p r) Hi'; try contradiction.
+            1: { (* i + 1 < p r not possible *)
+              rewrite order_fin_S in Hi. apply order_eq in Hi. pose proof Hi' as Hi''.
+              rewrite <- Hi in Hi''. rewrite order_flip in Hi''.
+              rewrite <- order_fin_S in Hi''. rewrite order_FS_LT in Hi''. inv Hi''.
+            }
+            (* i + 1 > p r *)
+            rewrite Hp. rewrite subtract_one_FS. reflexivity.
+      - (* i > p r *)
+        cases (q (FS i)) r Hqi; try contradiction.
+        + (* q (i + 1) < r *)
+          specialize (Hp (q' i)). rewrite Hq in *.
+          rewrite fin_S_not_highest, Hpq in Hp.
+          cases (not_highest (q (FS i)) r Hqi) r Hqi'.
+          2, 3: rewrite <- order_not_highest in Hqi'; rewrite Hqi in Hqi'; inv Hqi'.
+          cases (FS i) (p r) Hi'; try contradiction.
+          1: { (* i + 1 < p r is not possible *)
+            pose proof Hi' as Hi''. apply order_flip in Hi''.
+            apply order_GT_FS in Hi''. cbn in Hi''.
+            pose proof (order_transitive _ _ _ _ Hi Hi'').
+            rewrite order_reflexive in H. inv H.
+          }
+          (* i + 1 > p r *)
+          rewrite Hp. rewrite subtract_one_FS. reflexivity.
+        + (* q (i + 1) > r *)
+          specialize (Hp (q' i)). rewrite Hq in *.
+          rewrite FS_subtract_one, Hpq in Hp.
+          cases (subtract_one (q (FS i)) r Hqi) r Hqi'.
+          1: { (* q (i + 1) - 1 < r not possible *)
+            apply order_subtract_one_LT_inv in Hqi'.
+            destruct Hqi' as [Hqi' | Hqi']; rewrite Hqi in Hqi'; inv Hqi'.
+          }
+          * (* q (i + 1) - 1 = r *)
+            cases (FS i) (p r) Hi'; try contradiction.
+            1: { (* i + 1 < p r not possible *)
+              pose proof Hi' as Hi''. apply order_flip in Hi''.
+              apply order_GT_FS in Hi''. cbn in Hi''.
+              pose proof (order_transitive _ _ _ _ Hi Hi'').
+              rewrite order_reflexive in H. inv H.
+            }
+            (* i + 1 > p r *)
+            rewrite Hp. rewrite subtract_one_FS. reflexivity.
+          * (* q (i + 1) - 1 > r *)
+            cases (FS i) (p r) Hi'; try contradiction.
+            1: { (* i + 1 < p r not possible *)
+              pose proof Hi' as Hi''. apply order_flip in Hi''.
+              apply order_GT_FS in Hi''. cbn in Hi''.
+              pose proof (order_transitive _ _ _ _ Hi Hi'').
+              rewrite order_reflexive in H. inv H.
+            }
+            (* i + 1 > p r *)
+            rewrite Hp. rewrite subtract_one_FS. reflexivity.
+    }
+    {
+      intro i.
+      specialize (Hp i).
+      cases i r Hi.
+      - (* i < r *)
+        cases (p (fin_S i)) (p r) Hpi; try contradiction.
+        + (* p i < p r *)
+          specialize (Hq (p' i)). rewrite Hp in *.
+          rewrite fin_S_not_highest in Hq. do 2 rewrite Hqp in Hq.
+          cases (not_highest (p (fin_S i)) (p r) Hpi) (p r) Hpi'.
+          2, 3: rewrite <- order_not_highest in Hpi'; rewrite Hpi in Hpi'; inv Hpi'.
+          cases (fin_S i) r Hi'.
+          2, 3: rewrite order_fin_S in Hi; rewrite Hi' in Hi; inv Hi.
+          rewrite Hq. rewrite not_highest_fin_S. reflexivity.
+        + (* p i > p r *)
+          specialize (Hq (p' i)). rewrite Hp in *.
+          rewrite FS_subtract_one in Hq. do 2 rewrite Hqp in Hq.
+          cases (subtract_one (p (fin_S i)) (p r) Hpi) (p r) Hpi'.
+          1: { (* p i - 1 < p r not possible *)
+            pose proof Hpi as Hpi''. eapply order_subtract_one_GT_inv in Hpi''.
+            destruct Hpi'' as [Hpi'' | Hpi'']; rewrite Hpi' in Hpi''; inv Hpi''.
+          }
+          * (* p i - 1 = r *)
+            cases (fin_S i) r Hi'.
+            2, 3: rewrite order_fin_S in Hi; rewrite Hi' in Hi; inv Hi.
+            rewrite Hq. rewrite not_highest_fin_S. reflexivity.
+          * (* p i - 1 > r *)
+            cases (fin_S i) r Hi'.
+            2, 3: rewrite order_fin_S in Hi; rewrite Hi' in Hi; inv Hi.
+            rewrite Hq. rewrite not_highest_fin_S. reflexivity.
+      - (* i = r *)
+        cases (p (FS i)) (p r) Hpi; try contradiction.
+        + (* p (i + 1) < p r *)
+          specialize (Hq (p' i)). rewrite Hp in *.
+          rewrite fin_S_not_highest in Hq. do 2 rewrite Hqp in Hq.
+          cases (not_highest (p (FS i)) (p r) Hpi) (p r) Hpi'.
+          2, 3: rewrite <- order_not_highest in Hpi'; rewrite Hpi in Hpi'; inv Hpi'.
+          cases (FS i) r Hi'; try contradiction.
+          1: { (* i + 1 < r is not possible *)
+            rewrite order_fin_S in Hi. apply order_eq in Hi. pose proof Hi' as Hi''.
+            rewrite <- Hi in Hi''. rewrite order_flip in Hi''. rewrite <- order_fin_S in Hi''.
+            rewrite order_FS_LT in Hi''. inv Hi''.
+          }
+          (* i + 1 > r *)
+          rewrite Hq. rewrite subtract_one_FS. reflexivity.
+        + (* p (i + 1) > r *)
+          specialize (Hq (p' i)). rewrite Hp in *.
+          rewrite FS_subtract_one in Hq. do 2 rewrite Hqp in Hq.
+          cases (subtract_one (p (FS i)) (p r) Hpi) (p r) Hpi'.
+          1: { (* p (i + 1) - 1 < p r not possible *)
+            apply order_subtract_one_LT_inv in Hpi'.
+            destruct Hpi' as [Hpi' | Hpi']; rewrite Hpi in Hpi'; inv Hpi'.
+          }
+          * (* p (i + 1) - 1 = p r *)
+            cases (FS i) r Hi'; try contradiction.
+            1: { (* i + 1 < r not possible *)
+              rewrite order_fin_S in Hi. apply order_eq in Hi. pose proof Hi' as Hi''.
+              rewrite <- Hi in Hi''. rewrite order_flip in Hi''.
+              rewrite <- order_fin_S in Hi''. rewrite order_FS_LT in Hi''. inv Hi''.
+            }
+            (* i + 1 > r *)
+            rewrite Hq. rewrite subtract_one_FS. reflexivity.
+          * (* p (i + 1) - 1 > p r *)
+            cases (FS i) r Hi'; try contradiction.
+            1: { (* i + 1 < r not possible *)
+              rewrite order_fin_S in Hi. apply order_eq in Hi. pose proof Hi' as Hi''.
+              rewrite <- Hi in Hi''. rewrite order_flip in Hi''.
+              rewrite <- order_fin_S in Hi''. rewrite order_FS_LT in Hi''. inv Hi''.
+            }
+            (* i + 1 > r *)
+            rewrite Hq. rewrite subtract_one_FS. reflexivity.
+      - (* i > r *)
+        cases (p (FS i)) (p r) Hpi; try contradiction.
+        + (* p (i + 1) < p r *)
+          specialize (Hq (p' i)). rewrite Hp in *.
+          rewrite fin_S_not_highest in Hq. do 2 rewrite Hqp in Hq.
+          cases (not_highest (p (FS i)) (p r) Hpi) (p r) Hpi'.
+          2, 3: rewrite <- order_not_highest in Hpi'; rewrite Hpi in Hpi'; inv Hpi'.
+          cases (FS i) r Hi'; try contradiction.
+          1: { (* i + 1 < r is not possible *)
+            pose proof Hi' as Hi''. apply order_flip in Hi''.
+            apply order_GT_FS in Hi''. cbn in Hi''.
+            pose proof (order_transitive _ _ _ _ Hi Hi'').
+            rewrite order_reflexive in H. inv H.
+          }
+          (* i + 1 > r *)
+          rewrite Hq. rewrite subtract_one_FS. reflexivity.
+        + (* p (i + 1) > p r *)
+          specialize (Hq (p' i)). rewrite Hp in *.
+          rewrite FS_subtract_one in Hq. do 2 rewrite Hqp in Hq.
+          cases (subtract_one (p (FS i)) (p r) Hpi) (p r) Hpi'.
+          1: { (* p (i + 1) - 1 < p r not possible *)
+            apply order_subtract_one_LT_inv in Hpi'.
+            destruct Hpi' as [Hpi' | Hpi']; rewrite Hpi in Hpi'; inv Hpi'.
+          }
+          * (* p (i + 1) - 1 = p r *)
+            cases (FS i) r Hi'; try contradiction.
+            1: { (* i + 1 < r not possible *)
+              pose proof Hi' as Hi''. apply order_flip in Hi''.
+              apply order_GT_FS in Hi''. cbn in Hi''.
+              pose proof (order_transitive _ _ _ _ Hi Hi'').
+              rewrite order_reflexive in H. inv H.
+            }
+            (* i + 1 > r *)
+            rewrite Hq. rewrite subtract_one_FS. reflexivity.
+          * (* p (i + 1) - 1 > p r *)
+            cases (FS i) r Hi'; try contradiction.
+            1: { (* i + 1 < r not possible *)
+              pose proof Hi' as Hi''. apply order_flip in Hi''.
+              apply order_GT_FS in Hi''. cbn in Hi''.
+              pose proof (order_transitive _ _ _ _ Hi Hi'').
+              rewrite order_reflexive in H. inv H.
+            }
+            (* i + 1 > r *)
+            rewrite Hq. rewrite subtract_one_FS. reflexivity.
+    }
+  Qed.
+
+  Lemma remove_at_permutation_vectors {n X} `{Encode E} (v1 v2 : vec' (S n) (ctree E X)) i p q Hp Hq p' q'
+        (Hp' : p' = projT1 (remove_at_permutation p i Hp))
+        (Hq' : q' = projT1 (remove_at_permutation q (p i) Hq))
+        (Hpq : forall i, p (q i) = i)
+        (Hqp : forall i, q (p i) = i)
+        (Hpq' : forall i, p' (q' i) = i)
+        (Hqp' : forall i, q' (p' i) = i)
+        (Hsb1 : forall i, v1 i ~ v2 (p i))
+        (Hsb2 : forall i, v2 i ~ v1 (q i)) :
+    (forall j, remove_vec v1 i j ~ remove_vec v2 (p i) (p' j)) /\
+    (forall j, remove_vec v2 (p i) j ~ remove_vec v1 i (q' j)).
+  Proof.
+    split; intros j.
+    {
+      subst. destruct (remove_at_permutation p) as (p' & Hp'). cbn in *.
+      destruct (remove_at_permutation q) as (q' & Hq'). cbn in *. clear Hq'.
+      specialize (Hp' j).
+      cases j i Hj.
+      - (* j < i *)
+        rewrite <- remove_vec_index_before'; auto.
+        cases (p (fin_S j)) (p i) Hpj; try contradiction.
+        + (* p j < p i *)
+          rewrite <- remove_vec_index_before'; rewrite Hp'.
+          2: rewrite <- order_not_highest; auto.
+          rewrite fin_S_not_highest. auto.
+        + (* p j > p i *)
+          pose proof Hpj as Hpj'.
+          apply (order_subtract_one_GT_inv _ _ _ Hpj) in Hpj'.
+          destruct Hpj'; [rewrite <- remove_vec_index_eq' | rewrite <- remove_vec_index_after'];
+            rewrite Hp'; auto; rewrite FS_subtract_one; auto.
+      - (* j = i *)
+        rewrite <- remove_vec_index_eq'; auto.
+        cases (p (FS j)) (p i) Hpj; try contradiction.
+        + (* p (j + 1) < p i *)
+          rewrite <- remove_vec_index_before'; rewrite Hp'.
+          2: rewrite <- order_not_highest; auto.
+          rewrite fin_S_not_highest. auto.
+        + (* p (j + 1) > p i *)
+          pose proof Hpj as Hpj'.
+          apply (order_subtract_one_GT_inv _ _ _ Hpj) in Hpj'.
+          destruct Hpj'; [rewrite <- remove_vec_index_eq' | rewrite <- remove_vec_index_after'];
+            rewrite Hp'; auto; rewrite FS_subtract_one; auto.
+      - (* j > i *)
+        rewrite <- remove_vec_index_after'; auto.
+        cases (p (FS j)) (p i) Hpj; try contradiction.
+        + (* p (j + 1) < p i *)
+          rewrite <- remove_vec_index_before'; rewrite Hp'.
+          2: rewrite <- order_not_highest; auto.
+          rewrite fin_S_not_highest. auto.
+        + (* p (j + 1) > p i *)
+          pose proof Hpj as Hpj'.
+          apply (order_subtract_one_GT_inv _ _ _ Hpj) in Hpj'.
+          destruct Hpj'; [rewrite <- remove_vec_index_eq' | rewrite <- remove_vec_index_after'];
+            rewrite Hp'; auto; rewrite FS_subtract_one; auto.
+    }
+    {
+      subst. destruct (remove_at_permutation p) as (p' & Hp'). cbn in *. clear Hp'.
+      destruct (remove_at_permutation q) as (q' & Hq'). cbn in *.
+      specialize (Hq' j). rewrite Hqp in Hq'.
+      cases j (p i) Hj.
+      - (* j < p i *)
+        rewrite <- remove_vec_index_before'; auto.
+        cases (q (fin_S j)) i Hqj; try contradiction.
+        + (* q j < i *)
+          rewrite <- remove_vec_index_before'; rewrite Hq'.
+          2: rewrite <- order_not_highest; auto.
+          rewrite fin_S_not_highest. auto.
+        + (* q j > i *)
+          pose proof Hqj as Hqj'.
+          apply (order_subtract_one_GT_inv _ _ _ Hqj) in Hqj'.
+          destruct Hqj'; [rewrite <- remove_vec_index_eq' | rewrite <- remove_vec_index_after'];
+            rewrite Hq'; auto; rewrite FS_subtract_one; auto.
+      - (* j = p i *)
+        rewrite <- remove_vec_index_eq'; auto.
+        cases (q (FS j)) i Hqj; try contradiction.
+        + (* q (j + 1) < i *)
+          rewrite <- remove_vec_index_before'; rewrite Hq'.
+          2: rewrite <- order_not_highest; auto.
+          rewrite fin_S_not_highest. auto.
+        + (* q (j + 1) > i *)
+          pose proof Hqj as Hqj'.
+          apply (order_subtract_one_GT_inv _ _ _ Hqj) in Hqj'.
+          destruct Hqj'; [rewrite <- remove_vec_index_eq' | rewrite <- remove_vec_index_after'];
+            rewrite Hq'; auto; rewrite FS_subtract_one; auto.
+      - (* j > p i *)
+        rewrite <- remove_vec_index_after'; auto.
+        cases (q (FS j)) i Hqj; try contradiction.
+        + (* q (j + 1) < i *)
+          rewrite <- remove_vec_index_before'; rewrite Hq'.
+          2: rewrite <- order_not_highest; auto.
+          rewrite fin_S_not_highest. auto.
+        + (* q (j + 1) > i *)
+          pose proof Hqj as Hqj'.
+          apply (order_subtract_one_GT_inv _ _ _ Hqj) in Hqj'.
+          destruct Hqj'; [rewrite <- remove_vec_index_eq' | rewrite <- remove_vec_index_after'];
+            rewrite Hq'; auto; rewrite FS_subtract_one; auto.
+    }
+  Qed.
+End Ordering.
