theories/Lang/Yield.v
@@ -1,0 +1,699 @@
+From Coq Require Import
+     Arith.PeanoNat
+     Lists.List
+     Strings.String
+     Morphisms
+     Setoid
+     RelationClasses.
+
+From ExtLib Require Import
+     Data.String
+     Structures.Traversable
+     Data.Monads.StateMonad
+     Data.List
+     Data.Map.FMapAList.
+
+From Coinduction Require Import
+  coinduction rel tactics.
+
+From CTree Require Import
+  CTree.Core
+  Equ
+  SBisim
+  Lang.Vec
+  Lang.Par
+  CTree.Interp.State.
+
+From Equations Require Import Equations.
+
+Import ListNotations.
+Import CTreeNotations.
+
+Local Open Scope ctree_scope.
+Local Open Scope string_scope.
+
+Definition var : Set := string.
+
+(** For simplicity, the language manipulates [nat]s as values. *)
+Definition value : Type := nat.
+
+Inductive expr : Type :=
+| Lit (_ : value)
+| Var (_: var)
+| Plus  (_ _ : expr)
+| Minus (_ _ : expr)
+| Mult  (_ _ : expr).
+
+Inductive cond: Type :=
+| EqC (a b: expr)
+| LtC (a b: expr)
+| LeC (a b: expr).
+
+Inductive stmt : Type :=
+| Seq    (a b : stmt)            (* a ; b *)
+| Assign (x: var) (e: expr)      (* a := x *)
+| If     (i : cond) (t e : stmt) (* if (i) then { t } else { e } *)
+| While  (t : cond) (b : stmt)   (* while (t) { b } *)
+| Fork  (t1 t2 : stmt)           (* fork the current thread, first doing t1 in the inactive thread and t2 in the active thread *)
+| Skip                           (* ; *)
+| Yield                          (* yield *)
+.
+
+Variant memE : Type :=
+  | wr (id: var) (v: value): memE
+  | rd (id: var): memE.
+
+Global Instance encode_memE: Encode memE :=
+  fun e => match e with
+        | wr _ _ => unit
+        | rd _ => nat
+        end.
+
+Section Denote1.
+  Context (E := yieldE + forkE + memE).
+
+  Definition while (step : ctree E (unit + unit)) : ctree E unit :=
+    Ctree.iter (fun _ => step) tt.
+
+  Definition read (v: var) : ctree E nat :=
+    Ctree.trigger (rd v).
+  Definition write (v: var) (x: value) : ctree E unit :=
+    Ctree.trigger (wr v x).
+  
+  Program Definition yield : ctree E unit :=
+    @Ctree.trigger yieldE E _ _ _ _ Par.Yield.
+  Next Obligation.
+    exact unit.
+  Defined.
+  Next Obligation.
+    exact (inl (inl Par.Yield)).
+  Defined.  
+
+  Program Definition fork : ctree E bool :=
+    @Ctree.trigger forkE E _ _ _ _ Par.Fork.
+  Next Obligation.
+    exact bool.
+  Defined.
+  Next Obligation.
+    exact (inl (inr Par.Fork)).
+  Defined.
+
+
+  Fixpoint denote_expr (e : expr) : ctree E value :=
+    match e with
+    | Var v     => x <- read v ;; yield;; Ret x
+    | Lit n     => Ret n
+    | Plus a b  => l <- denote_expr a ;; r <- denote_expr b ;; Ret (l + r)%nat
+    | Minus a b => l <- denote_expr a ;; r <- denote_expr b ;; Ret (l - r)%nat
+    | Mult a b  => l <- denote_expr a ;; r <- denote_expr b ;; Ret (l * r)%nat
+    end.
+
+  Definition denote_cond (c: cond): ctree E bool :=
+    match c with
+    | EqC l r =>
+        vl <- denote_expr l ;;
+        vr <- denote_expr r ;;
+        Ret (vl =? vr)%nat
+    | LeC l r =>
+        vl <- denote_expr l ;;
+        vr <- denote_expr r ;;
+        Ret (vl <=? vr)%nat
+    | LtC l r =>
+        vl <- denote_expr l ;;
+        vr <- denote_expr r ;;
+        Ret (vl <? vr)%nat
+    end.
+  
+  Fixpoint denote_imp (s : stmt) : thread :=
+    match s with
+    | Assign x e =>  v <- denote_expr e ;; u <- write x v ;; Ret u
+    | Seq a b    =>  denote_imp a ;; denote_imp b
+    | If i t e   =>
+        v <- denote_expr i ;;
+        if is_true v then denote_imp t else denote_imp e
+
+    | While t b =>
+        while (v <- denote_expr t ;;
+	           if is_true v
+               then denote_imp b ;; Ret (inl tt)
+               else ret (inr tt))
+
+    | Fork t1 t2 =>
+        b <- fork;;
+        match b with
+        | true => denote_imp t1
+        | false => denote_imp t2
+        end
+    | Skip => Ret tt
+    | YieldS => yield
+    end.
+
+  Definition interp_concurrency (t : stmt) : completed :=
+    schedule 1 (fun _ => denote_imp t) (Some Fin.F1).
+
+  (* specific case for ctree rather than generic monad M *)
+  #[global] Instance MonadBr_stateT {S E} : Utils.MonadBr (Monads.stateT S (ctree E)) :=
+    fun b n s =>
+      f <- mbr b n;;
+      ret (s, f).
+
+  Definition handle_spawn : (yieldE +' spawnE +' MemE) ~> ctree (yieldE +' MemE) :=
+    fun _ e =>
+      match e with
+      | inl1 y => trigger y
+      | inr1 (inl1 s) => match s with Spawn => ret tt end (* erase spawn events *)
+      | inr1 (inr1 m) => trigger m
+      end.
+
+  Definition interp_spawn : completed -> ctree (yieldE +' MemE) unit :=
+    interp handle_spawn (T:=unit).
+
+  Definition handle_yield : (yieldE +' MemE) ~> ctree MemE :=
+    fun _ e =>
+      match e with
+      | inl1 s => match s with Yield => ret tt end (* erase yield events *)
+      | inr1 m => trigger m
+      end.
+
+  Definition interp_yield : ctree (yieldE +' MemE) unit -> ctree MemE unit :=
+    interp handle_yield (T:=unit).
+
+  (* list of key value pairs *)
+  Definition env := alist var value.
+
+  Definition handle_state : MemE ~> Monads.stateT env (ctree void1) :=
+    fun _ e s =>
+      match e with
+      | rd x => Ret (s, lookup_default x 0%nat s)
+      | wr x v => Ret (Maps.add x v s, tt)
+      end.
+
+  Definition interp_imp (t : stmt) : Monads.stateT env (ctree void1) unit :=
+    interp_state handle_state (interp_yield (interp_spawn (interp_concurrency t))).
+
+  Lemma denote_expr_bounded e :
+    brD_bound 1 (denote_expr e).
+  Proof.
+    induction e; cbn; unfold trigger; auto.
+    - step. rewrite bind_vis. constructor. intros.
+      step. rewrite bind_ret_l. rewrite bind_vis. constructor. intros.
+      step. rewrite bind_ret_l. constructor.
+    - step. constructor.
+    - apply bind_brD_bound; auto.
+      intros. apply bind_brD_bound; auto.
+      intros. step. constructor.
+    - apply bind_brD_bound; auto.
+      intros. apply bind_brD_bound; auto.
+      intros. step. constructor.
+    - apply bind_brD_bound; auto.
+      intros. apply bind_brD_bound; auto.
+      intros. step. constructor.
+  Qed.
+
+  Lemma denote_imp_bounded t :
+    brD_bound 1 (denote_imp t).
+  Proof.
+    induction t; cbn.
+    - apply bind_brD_bound. apply denote_expr_bounded. intros.
+      step. rewrite bind_trigger. constructor. intros.
+      step. constructor.
+    - apply bind_brD_bound; auto.
+    - apply bind_brD_bound. apply denote_expr_bounded.
+      intros. step. step in IHt1. step in IHt2. destruct (is_true x); auto.
+    - unfold while. apply iter_brD_bound; auto.
+      intros. apply bind_brD_bound. apply denote_expr_bounded.
+      intros. destruct (is_true x).
+      + apply bind_brD_bound; auto.
+        intros. step. constructor.
+      + step. constructor.
+    - apply bind_brD_bound.
+      + intros. step. constructor. intros. step. constructor.
+      + intros. destruct x; auto.
+    - step. constructor.
+    - step. constructor. intros. step. constructor.
+  Qed.
+
+  Lemma schedule_forks_equ t1 t2 :
+    (schedule 1 (fun _ : fin 1 => denote_imp (Fork t1 (Fork t2 Skip))) (Some Fin.F1))
+      ≅
+    trigger Spawn;;
+    trigger Spawn;;
+    (Guard (schedule 2
+                     (cons_vec
+                        (denote_imp t2)
+                        (fun _ => denote_imp t1))
+                     None)).
+  Proof.
+    rewrite rewrite_schedule. simp schedule_match.
+    cbn. CTree.fold_subst.
+    unfold trigger.
+    step. cbn. constructor. intros [].
+
+    rewrite rewrite_schedule. simp schedule_match. simp cons_vec.
+    unfold replace_vec. cbn.
+    step. cbn. constructor. intros [].
+
+    rewrite rewrite_schedule. simp schedule_match. simp cons_vec. cbn.
+    step. cbn. constructor. intros _.
+
+    apply equ_schedule. intro i.
+    dependent destruction i.
+    - simp remove_vec. simp cons_vec. CTree.fold_subst.
+      rewrite bind_ret_l. reflexivity.
+    - dependent destruction i; [| inv i].
+      simp remove_vec. simp cons_vec.
+      unfold remove_front_vec. simp cons_vec. cbn. simp cons_vec.
+      rewrite bind_ret_l. reflexivity.
+  Qed.
+
+  Equations p : fin 2 -> fin 2 :=
+    p Fin.F1 := Fin.FS Fin.F1;
+    p (Fin.FS Fin.F1) := Fin.F1.
+
+  Lemma p_inverse : forall i, p (p i) = i.
+  Proof.
+    intros. dependent destruction i.
+    - simp p; auto.
+    - dependent destruction i. simp p; auto. inv i.
+  Qed.
+
+  Lemma schedule_order (t1 t1' t2 t2' : ctree E unit)
+    (Hbound1 : brD_bound 1 t1)
+    (Hbound2 : brD_bound 1 t2)
+    (Hbound1' : brD_bound 1 t1')
+    (Hbound2' : brD_bound 1 t2')
+    (Ht1 : t1 ~ t1')
+    (Ht2 : t2 ~ t2') :
+    BrS 2 (fun i' : fin 2 =>
+                 schedule 2
+                          (cons_vec t1 (fun _ => t2))
+                          (Some i')) ~
+    BrS 2 (fun i' : fin 2 =>
+                 schedule 2
+                          (cons_vec t2' (fun _ => t1'))
+                          (Some i')).
+  Proof.
+    apply sb_brS; intros i; exists (p i); [| symmetry];
+      apply schedule_permutation with (q:=p);
+      try solve [intros i0; dependent destruction i0; simp cons_vec];
+      try solve [apply p_inverse];
+      try solve [ intros i0; dependent destruction i0;
+                  [| dependent destruction i0; [| inv i0]]; simp p; simp cons_vec; auto];
+      try solve [ intros i0; dependent destruction i0;
+                  [| dependent destruction i0; [| inv i0]]; simp p; simp cons_vec; symmetry; auto].
+  Qed.
+
+  Lemma schedule_order' (t1 t1' t2 t2' : ctree E unit)
+    (Hbound1 : brD_bound 1 t1)
+    (Hbound2 : brD_bound 1 t2)
+    (Hbound1' : brD_bound 1 t1')
+    (Hbound2' : brD_bound 1 t2')
+    (Ht1 : t1 ~ t1')
+    (Ht2 : t2 ~ t2') :
+    BrD 2 (fun i' : fin 2 =>
+                 schedule 2
+                          (cons_vec t1 (fun _ => t2))
+                          (Some i')) ~
+    BrD 2 (fun i' : fin 2 =>
+                 schedule 2
+                          (cons_vec t2' (fun _ => t1'))
+                          (Some i')).
+  Proof.
+    apply sb_brD; intros i; exists (p i); [| symmetry];
+      apply schedule_permutation with (q:=p);
+      try solve [intros i0; dependent destruction i0; simp cons_vec];
+      try solve [apply p_inverse];
+      try solve [ intros i0; dependent destruction i0;
+                  [| dependent destruction i0; [| inv i0]]; simp p; simp cons_vec; auto];
+      try solve [ intros i0; dependent destruction i0;
+                  [| dependent destruction i0; [| inv i0]]; simp p; simp cons_vec; symmetry; auto].
+  Qed.
+
+  Lemma schedule_order'' (t1 t1' t2 t2' : ctree E unit)
+        (Hbound1 : brD_bound 1 t1)
+        (Hbound2 : brD_bound 1 t2)
+        (Hbound1' : brD_bound 1 t1')
+        (Hbound2' : brD_bound 1 t2')
+        (Ht1 : t1 ~ t1')
+        (Ht2 : t2 ~ t2') :
+    schedule 2 (cons_vec t1 (fun _ => t2)) None ~
+    schedule 2 (cons_vec t2' (fun _ => t1')) None.
+  Proof.
+    do 2 rewrite rewrite_schedule. simp schedule_match.
+    apply sb_vis. intros. apply schedule_order'; auto.
+  Qed.
+
+  Lemma commut_forks s1 s2 :
+    interp_concurrency (Fork s1 (Fork s2 Skip)) ~
+    interp_concurrency (Fork s2 (Fork s1 Skip)).
+  Proof.
+    unfold interp_concurrency.
+    do 2 rewrite schedule_forks_equ.
+    unfold trigger.
+    (* not sure why we can't just rewrite twice, but we can below *)
+    rewrite bind_vis. symmetry. rewrite bind_vis.
+    apply sb_vis. intros []. do 2 rewrite bind_ret_l.
+    do 2 rewrite bind_vis.
+    apply sb_vis. intros []. do 2 rewrite bind_ret_l.
+    apply sb_guard_lr.
+
+    do 2 rewrite rewrite_schedule. simp schedule_match.
+    apply sb_vis. intros [].
+    apply schedule_order'; try solve [apply denote_imp_bounded]; reflexivity.
+  Qed.
+
+  Lemma fork_skip_equ s :
+    interp_concurrency (Fork s Skip)
+                       ≅
+    trigger Spawn;;
+    Guard (Ret tt);;
+    trigger Yield;;
+    Guard (interp_concurrency s).
+  Proof.
+    unfold interp_concurrency. cbn.
+
+    rewrite rewrite_schedule. simp schedule_match.
+    cbn. unfold trigger.
+    rewrite replace_vec_unary.
+    step. cbn. constructor. intros [].
+
+    rewrite rewrite_schedule. simp schedule_match.
+    CTree.fold_subst. rewrite (bind_ret_l tt).
+    simp cons_vec. cbn. rewrite remove_vec_cons_2.
+    step. cbn. constructor. intros _.
+
+    rewrite rewrite_schedule. simp schedule_match.
+    CTree.fold_subst. rewrite (bind_ret_l tt).
+    step. cbn. constructor. intros [].
+
+    CTree.fold_subst. rewrite (bind_ret_l tt).
+    step. constructor.
+    dependent destruction i. 2: inv i.
+    apply equ_schedule. repeat intro. rewrite bind_ret_l. reflexivity.
+  Qed.
+
+  Lemma yield_equ s :
+    interp_concurrency (Seq YieldS s) ≅
+                       Guard (Ret tt);;
+    trigger Yield;;
+    Guard (interp_concurrency s).
+  Proof.
+    unfold interp_concurrency. cbn.
+
+    rewrite rewrite_schedule. simp schedule_match.
+    cbn. CTree.fold_subst.
+    rewrite replace_vec_unary.
+    step. cbn. constructor. intros _.
+    CTree.fold_subst.
+
+    rewrite rewrite_schedule. simp schedule_match.
+    step. cbn. constructor.
+    intros [].
+
+    CTree.fold_subst.
+    step. cbn. constructor.
+    dependent destruction i. 2: inv i.
+    apply equ_schedule. repeat intro. rewrite bind_ret_l. reflexivity.
+  Qed.
+
+  (* first one has one more yield *)
+  Lemma yield_yield_fork s :
+    interp_yield (interp_spawn (interp_concurrency (Seq YieldS (Seq YieldS s)))) ~
+    interp_yield (interp_spawn (interp_concurrency (Fork s Skip))).
+  Proof.
+    rewrite yield_equ, fork_skip_equ.
+    unfold interp_yield, interp_spawn.
+
+    unfold trigger.
+    do 2 rewrite interp_bind. do 2 rewrite interp_tau. setoid_rewrite interp_tau.
+    symmetry. do 2 rewrite interp_bind. rewrite interp_vis.
+    cbn. rewrite bind_ret_l. rewrite interp_tau.
+    apply sbisim_clo_bind. { do 2 apply sb_guard_r. do 2 apply sb_guard_lr. reflexivity. }
+    intros [].
+
+    do 2 rewrite interp_bind. do 2 rewrite interp_tau. setoid_rewrite interp_tau.
+    symmetry. do 2 (rewrite bind_Guard; apply sb_guard_r). do 2 setoid_rewrite interp_ret.
+    do 2 rewrite interp_bind. rewrite interp_vis. cbn.
+    rewrite interp_bind. unfold trigger. rewrite interp_vis. cbn. rewrite bind_ret_l.
+    rewrite bind_Guard.
+    apply sbisim_clo_bind.
+    {
+      apply sb_guard_lr. rewrite interp_ret. rewrite bind_ret_l.
+      rewrite interp_tau. apply sb_guard_lr, sb_guard_l.
+      do 2 rewrite interp_ret. reflexivity.
+    }
+    intros [].
+
+    do 2 rewrite interp_tau. symmetry.
+    do 2 rewrite interp_bind. rewrite interp_vis. cbn. unfold trigger.
+    rewrite interp_bind. rewrite interp_vis. cbn.
+    rewrite bind_ret_l. rewrite bind_Guard.
+    setoid_rewrite interp_ret. setoid_rewrite bind_ret_l.
+    setoid_rewrite interp_tau.
+    setoid_rewrite interp_ret.
+    do 3 (rewrite bind_Guard; apply sb_guard_lr). rewrite bind_ret_l.
+    rewrite interp_tau.
+    apply sb_guard_lr. apply sb_guard_l.
+    rewrite interp_tau.
+    do 2 apply sb_guard_l.
+    rewrite yield_equ.
+
+    symmetry. do 2 rewrite interp_bind. do 2 rewrite interp_tau. setoid_rewrite interp_tau.
+    do 2 setoid_rewrite interp_ret.
+    do 4 (rewrite bind_Guard; apply sb_guard_l). rewrite bind_ret_l.
+
+    do 2 rewrite interp_bind. unfold trigger.
+    rewrite interp_vis. cbn. unfold trigger. rewrite interp_bind.
+    rewrite interp_vis. cbn. rewrite bind_ret_l. setoid_rewrite interp_ret.
+    do 2 rewrite bind_Guard. apply sb_guard_l. rewrite bind_ret_l.
+    rewrite interp_tau.
+    do 2 (rewrite bind_Guard; apply sb_guard_l).
+    rewrite interp_ret. rewrite bind_ret_l.
+
+    do 2 rewrite interp_tau. setoid_rewrite interp_tau. do 4 apply sb_guard_l. reflexivity.
+  Qed.
+
+  Lemma fork_skip_yield s :
+    interp_spawn (interp_concurrency (Seq YieldS s)) ~
+    interp_spawn (interp_concurrency (Fork s Skip)).
+  Proof.
+    rewrite yield_equ, fork_skip_equ.
+    unfold interp_spawn.
+
+    rewrite interp_bind. rewrite interp_tau.
+    unfold trigger.
+    symmetry. rewrite interp_bind. rewrite interp_vis.
+    cbn. rewrite bind_ret_l.
+    apply sbisim_clo_bind. { apply sb_guard_r. reflexivity. }
+    intros [].
+
+    rewrite interp_bind. rewrite interp_tau.
+    symmetry. do 2 (rewrite bind_Guard; apply sb_guard_r).
+    symmetry. rewrite interp_ret. rewrite bind_ret_l.
+    reflexivity.
+  Qed.
+
+  Lemma spawn_skip s :
+    interp_yield (interp_spawn (interp_concurrency (Fork s Skip))) ~
+    interp_yield (interp_spawn (interp_concurrency s)).
+  Proof.
+    rewrite fork_skip_equ.
+    unfold interp_yield, interp_spawn.
+
+    unfold trigger. do 2 rewrite interp_bind. rewrite interp_vis. cbn.
+    rewrite bind_ret_l. rewrite interp_tau.
+    do 2 (rewrite bind_Guard; apply sb_guard_l).
+    do 2 rewrite interp_ret. rewrite bind_ret_l.
+
+    do 2 rewrite interp_bind. do 2 rewrite interp_tau. setoid_rewrite interp_tau.
+    do 4 (rewrite bind_Guard; apply sb_guard_l).
+    do 2 rewrite interp_ret. rewrite bind_ret_l.
+
+    do 2 rewrite interp_bind. rewrite interp_vis. cbn.
+    unfold trigger. rewrite interp_bind. rewrite interp_vis.
+    cbn. rewrite bind_ret_l. cbn.
+    do 2 rewrite bind_Guard. apply sb_guard_l.
+    rewrite interp_ret. rewrite bind_ret_l.
+    rewrite interp_tau.
+    do 2 (rewrite bind_Guard; apply sb_guard_l).
+    do 2 rewrite interp_ret. rewrite bind_ret_l.
+
+    do 2 rewrite interp_tau. setoid_rewrite interp_tau.
+    do 4 apply sb_guard_l.
+    reflexivity.
+  Qed.
+
+  Lemma while_true_unfold_sbisim s1 :
+    denote_imp (While (Lit 1%nat) s1) ~ denote_imp s1;; denote_imp (While (Lit 1%nat) s1).
+  Proof.
+    cbn. unfold while. rewrite unfold_iter at 1.
+    rewrite bind_ret_l. unfold is_true.
+    assert ((1 =? 0)%nat = false) by reflexivity.
+    rewrite H. unfold E. rewrite bind_bind.
+    apply sbisim_clo_bind. reflexivity.
+    intros _. rewrite bind_ret_l. apply sb_guard.
+  Qed.
+
+  Lemma commut_forks_unfold s :
+    interp_concurrency (Fork (While (Lit 1%nat) YieldS) (Fork s Skip)) ~
+    interp_concurrency (Fork s (Fork (Seq YieldS (While (Lit 1%nat) YieldS)) Skip)).
+  Proof.
+    unfold interp_concurrency.
+    do 2 rewrite schedule_forks_equ.
+    apply sbisim_clo_bind. reflexivity. intros _.
+    apply sbisim_clo_bind. reflexivity. intros _.
+    apply sb_guard_lr.
+
+    apply schedule_order''; try solve [apply denote_imp_bounded]; try reflexivity.
+    apply while_true_unfold_sbisim.
+  Qed.
+
+  Lemma assign_equ :
+    interp_concurrency (Assign "x" (Lit 2)) ≅
+                       (vis (wr "x" 2) (fun _ => Guard (ret tt))).
+  Proof.
+    unfold interp_concurrency. cbn.
+
+    rewrite rewrite_schedule. simp schedule_match.
+    cbn. CTree.fold_subst.
+    step. constructor. intros [].
+
+    rewrite rewrite_schedule. simp schedule_match.
+    cbn. step. constructor. intros _.
+
+    rewrite rewrite_schedule. simp schedule_match. reflexivity.
+  Qed.
+
+  Lemma fork_assign_assign_equ :
+    interp_concurrency (Fork (Assign "x" (Lit 2))
+                             (Assign "x" (Lit 1%nat))) ≅
+                       trigger Spawn;; (vis (wr "x" 1%nat) (fun _ => (Guard (trigger Yield;; Guard ((vis (wr "x" 2) (fun _ => Guard (ret tt)))))))).
+  Proof.
+    unfold interp_concurrency. cbn.
+
+    rewrite rewrite_schedule. simp schedule_match.
+    cbn. CTree.fold_subst.
+    rewrite replace_vec_unary.
+    step. cbn. constructor. intros [].
+
+    rewrite rewrite_schedule. simp schedule_match.
+    CTree.fold_subst.
+    simp cons_vec. cbn.
+    step. cbn. constructor. intros [].
+
+    rewrite rewrite_schedule. simp schedule_match.
+    rewrite replace_vec_cons_2.
+    step. constructor. intros _.
+
+    rewrite rewrite_schedule. simp schedule_match.
+    step. cbn. constructor. CTree.fold_subst. intros [].
+
+    step. cbn. constructor. intros i.
+
+    dependent destruction i. 2: inv i.
+    rewrite remove_vec_cons_2.
+    rewrite rewrite_schedule. simp schedule_match. cbn.
+    step. constructor. intros [].
+
+    rewrite rewrite_schedule. simp schedule_match. cbn.
+    step. constructor. intros _.
+
+    rewrite rewrite_schedule. simp schedule_match. reflexivity.
+  Qed.
+
+  Lemma filter_filter : forall {A} f (l : list A), filter f (filter f l) = filter f l.
+  Proof.
+    intros. induction l.
+    - reflexivity.
+    - cbn. destruct (f a) eqn:?.
+      + cbn. rewrite Heqb. f_equal. apply IHl.
+      + apply IHl.
+  Qed.
+
+  Lemma alist_add_alist_add : forall {K RD_K V}, RelDec.RelDec_Correct (RD_K) ->
+                                            forall k v v' l, @alist_add K eq RD_K V k v (alist_add _ k v' l) = alist_add _ k v l.
+  Proof.
+    intros. unfold alist_add, alist_remove. cbn. rewrite filter_filter.
+    rewrite RelDec.rel_dec_eq_true; auto.
+  Qed.
+
+  Lemma interp_fork_assign_assign s :
+    interp_imp (Fork (Assign "x" (Lit 2))
+                             (Assign "x" (Lit 1%nat))) s ~
+    interp_imp (Assign "x" (Lit 2)) s.
+  Proof.
+    unfold interp_imp.
+    rewrite fork_assign_assign_equ, assign_equ.
+    unfold interp_yield, interp_spawn.
+
+    rewrite interp_bind. unfold trigger. rewrite interp_vis.
+    cbn. rewrite bind_ret_l. setoid_rewrite interp_ret.
+    rewrite interp_bind.
+    cbn. rewrite interp_tau. setoid_rewrite interp_ret.
+
+    do 2 rewrite unfold_interp_state. cbn.
+    rewrite bind_ret_l.
+    apply sb_guard_lr. apply sb_guard_l.
+
+    do 2 rewrite unfold_interp_state. cbn.
+    do 2 apply sb_guard_lr. rewrite unfold_interp_state. cbn.
+    rewrite bind_ret_l. apply sb_guard_l.
+
+    (* push the yield and spawn interps all the way down *)
+    CTree.fold_subst. repeat rewrite bind_ret_l.
+    setoid_rewrite interp_bind. cbn. setoid_rewrite bind_ret_l.
+    setoid_rewrite interp_ret.
+    setoid_rewrite bind_ret_l.
+    repeat setoid_rewrite interp_tau.
+    setoid_rewrite interp_bind.
+    setoid_rewrite interp_vis.
+    do 2 setoid_rewrite interp_bind.
+    setoid_rewrite interp_vis. cbn.
+    setoid_rewrite bind_ret_l.
+    setoid_rewrite interp_ret.
+    setoid_rewrite interp_tau.
+    setoid_rewrite interp_ret.
+    repeat setoid_rewrite interp_tau.
+    setoid_rewrite bind_Guard.
+    setoid_rewrite bind_ret_l.
+    repeat setoid_rewrite bind_Guard.
+    setoid_rewrite bind_ret_l.
+
+    do 6 (do 2 rewrite unfold_interp_state; cbn; do 2 apply sb_guard_lr).
+    do 8 (rewrite unfold_interp_state; cbn; do 2 apply sb_guard_l).
+
+    do 2 rewrite unfold_interp_state. cbn.
+    rewrite bind_ret_l.
+    apply sb_guard_l.
+    CTree.fold_subst. cbn. repeat rewrite bind_ret_l.
+
+    rewrite unfold_interp_state. cbn.
+    do 2 apply sb_guard_l.
+
+    rewrite unfold_interp_state. cbn.
+    CTree.fold_subst. setoid_rewrite bind_bind. do 2 setoid_rewrite bind_ret_l.
+    do 2 apply sb_guard_l.
+
+    rewrite unfold_interp_state. cbn.
+    do 2 apply sb_guard_l.
+
+    rewrite unfold_interp_state. cbn.
+    CTree.fold_subst. repeat setoid_rewrite bind_ret_l.
+    do 2 apply sb_guard_l.
+
+    rewrite unfold_interp_state. cbn.
+    do 2 apply sb_guard_l.
+
+    rewrite unfold_interp_state. cbn.
+    CTree.fold_subst. setoid_rewrite bind_bind. do 2 setoid_rewrite bind_ret_l.
+    do 2 apply sb_guard_l.
+
+    rewrite unfold_interp_state. cbn.
+    do 2 apply sb_guard_l.
+
+    rewrite unfold_interp_state. cbn.
+
+    rewrite alist_add_alist_add. 2: apply RelDec_Correct_string. reflexivity.
+  Qed.
+
+End Denote1.
